\subsection*{Exercise 1.1.8}

\subsubsection{Instruction}

Find the below values for the function $ f(x) = 4x^2 - 3x + 1 $, if they exist, then simplify.
\begin{enumerate}[label=(\alph*)]
  \item $ f(0) $.
  \item $ f(1) $.
  \item $ f(3) $.
  \item $ f(-x) $.
  \item $ f(a) $.
  \item $ f(a + h) $.
\end{enumerate}

\subsubsection{Solution}

\begin{enumerate}[label=(\alph*)]
  \item $ f(0) = 4 \cdot 0^2 - 3 \cdot 0 + 1 = 4 \cdot 0 - 0 + 1 = 0 - 0 + 1 = 1 $.
  \item $ f(1) = 4 \cdot 1^2 - 3 \cdot 1 + 1 = 4 \cdot 1 - 3 + 1 = 4 - 3 + 1 = 2 $.
  \item $ f(3) = 4 \cdot 3^2 - 3 \cdot 3 + 1 = 4 \cdot 9 - 9 + 1 = 36 - 9 + 1 = 28 $.
  \item $ f(-x) = 4(-x)^2 - 3(-x) + 1 = 4x^2 + 3x + 1 $.
  \item $ f(a) = 4a^2 - 3a + 1 $.
  \item
    \(
      \begin{aligned}[t]
        f(a + h) &= 4(a + h)^2 - 3(a + h) + 1 \\
        &= 4(a^2 + 2ah + h^2) - 3a - 3h + 1 \\
        &= 4a^2 + 4h^2 + 8ah -3a - 3h + 1.
      \end{aligned}
    \)

\end{enumerate}

\subsubsection{Answer}

\begin{enumerate}[label=(\alph*)]
  \item $ 1 $.
  \item $ 2 $.
  \item $ 28 $.
  \item $ 4x^2 + 3x + 1 $.
  \item $ 4a^2 - 3a + 1 $.
  \item $ 4a^2 + 4h^2 + 8ah -3a - 3h + 1 $.
\end{enumerate}
